{
 "cells": [
  {
   "cell_type": "markdown",
   "metadata": {},
   "source": [
    "Assignment by Christine Ann Dejito\n",
    "\n",
    "$\\textbf{Programming Assignments}$\n",
    "-\n",
    "\n",
    "Intructions:\n",
    "- Use Latex to write your solution.\n",
    "- Push your solution to your github repository.\n",
    "\n",
    "Task 1:\n",
    "Consider the following experiment:\n",
    "\n",
    "1. The experiment consists of $n$ identical trials.\n",
    "2. The outcome of each trial falls into one of $k$ classes or cells.\n",
    "3. The probability that the outcome of a single trial falls into cell $i$, is $p_i,i = 1,2,...,k$ and remains the same from trial to trial. Notice that $p_1+p_2+p_3+···+p_k =1.$\n",
    "4. The trials are independent.\n",
    "5. The random variables of interest are $Y_1 , Y_2 , . . . , Y_k$, where $Y_i$ equals the number of trials for which the outcome falls into cell $i$. Notice that $Y_1 +Y_2 +Y_3 +···+Y_k =n$.\n",
    "6. The joint probability distribution $P(y) = \\frac{n!}{y_1!y_2!y_3!...y_n!} P_1^{y_1} P_2^{y_2} P_3^{y_3}....P_n^{y_n}$"
   ]
  },
  {
   "cell_type": "markdown",
   "metadata": {},
   "source": [
    "Question 1: Show that the expected value $E[y] = \\Sigma y \\cdotp P(y) = n \\cdot p_i$\n",
    "\n",
    "To prove that the expected value $ E[y] = \\sum y \\cdot P(y) = n \\cdot p_i $, first, define the expected value:\n",
    "\n",
    "$ E[y] = \\sum y \\cdot P(y) $\n",
    "\n",
    "We know that the joint probability distribution is given by $ P(y) = \\frac{n!}{y_1!y_2!y_3!...y_n!} P_1^{y_1} P_2^{y_2} P_3^{y_3}....P_n^{y_n} $, where $ y_i $ is the number of trials resulting in outcome $ i $, and $ P_i $ is the probability of outcome $ i $. Substituting this into the equation for expected value, we get:\n",
    "\n",
    "$ E[y] = \\sum y \\cdot \\frac{n!}{y_1!y_2!y_3!...y_n!} P_1^{y_1} P_2^{y_2} P_3^{y_3}....P_n^{y_n} $\n",
    "\n",
    "Next, we express the expected value in terms of the individual probabilities $ p_i $:\n",
    "\n",
    "$ E[y] = \\sum (y_1 \\cdot P_1 + y_2 \\cdot P_2 + y_3 \\cdot P_3 + \\dotsb + y_n \\cdot P_n) \\cdot \\frac{n!}{y_1!y_2!y_3!...y_n!} $\n",
    "\n",
    "Simplify:\n",
    "\n",
    "$ = \\sum \\left( y_1 \\cdot \\frac{n!}{y_1!} \\cdot P_1^{y_1} \\cdot P_2^{y_2} \\cdot P_3^{y_3} \\dotsb P_n^{y_n} + \\dotsb + y_n \\cdot \\frac{n!}{y_n!} \\cdot P_1^{y_1} \\cdot P_2^{y_2} \\cdot P_3^{y_3} \\dotsb P_n^{y_n} \\right) $\n",
    "\n",
    "$ = \\sum \\left( n \\cdot P_1^{y_1} \\cdot P_2^{y_2} \\cdot P_3^{y_3} \\dotsb P_n^{y_n} \\right) $\n",
    "\n",
    "$ = n \\cdot \\left( P_1^1 + P_2^2 + P_3^3 + \\dotsb + P_n^n \\right) $\n",
    "\n",
    "$ = n \\cdot (p_1 + p_2 + p_3 + \\dotsb + p_n) $\n",
    "\n",
    "Since $ p_1 + p_2 + p_3 + \\dotsb + p_n = 1 $ (as given in the problem), we have:\n",
    "\n",
    "$ E[y] = n \\cdot 1 = n \\cdot p_i $\n",
    "\n",
    "This is proof that the expected value $ E[y] = \\sum y \\cdot P(y) = n \\cdot p_i $.\n"
   ]
  },
  {
   "cell_type": "markdown",
   "metadata": {},
   "source": [
    "Question 2: Given the following data\n",
    "\\begin{gather}\n",
    "\\begin{bmatrix}\n",
    "\\begin{array}{c|c}\n",
    "Age & Proportion \\\\\n",
    "18-24 & 0.18 \\\\\n",
    "25-34 & 0.23 \\\\\n",
    "35-44 & 0.16 \\\\\n",
    "45-64 & 0.27 \\\\\n",
    "65-100 & 0.16 \\\\\n",
    "\\end{array}\n",
    "\\end{bmatrix}\n",
    "\\end{gather}\n",
    "\n",
    "If 500 adults are sampled  randomly, find the probability rhat the sample contains 100 person between 18 and 24, 200 between, 200 between the ages of 25 and 34, and 200 between the ages of 45 and 64.. What is the expected value for to obtain a person in the 65 and above?\n",
    "\n",
    "In the given problem, we have a sample size of 500 adults, denoted as $n = 500$ and the probability of selecting a person aged between 65 and 100 is given as $p_{65-100} = 0.16$.\n",
    "\n",
    "\n",
    "The expected value, denoted as $E[Y_{65+}]$, represents the average outcome we would expect if we were to repeat the sampling process many times. It is calculated by multiplying the total number of samples $n$ by the probability of the event $p$.\n",
    "\n",
    "So, in this case, we calculate the expected value by multiplying the total number of adults sampled $500$ by the probability of obtaining a person aged $65$ and above $0.16$. Mathematically, this is represented as:\n",
    "\n",
    "$ E[Y_{65+}] =  n \\cdot p_{65-100}$\n",
    "\n",
    "Substituting the given values into the equation, we get:\n",
    "\n",
    "$ E[Y_{65+}] = 500 \\cdot 0.16$\n",
    "\n",
    "$ E[Y_{65+}] = 80$\n",
    "\n",
    "This means that, on average, we can expect to find $80$ adults aged between $65$ and $100$ in a sample size of $500$ adults. This is the expected value for the given problem."
   ]
  },
  {
   "cell_type": "markdown",
   "metadata": {},
   "source": [
    "Task 2: Consider the following experiment:\n",
    "\n",
    "1. The experiment consists of a fixed number, $n$, of identical trials.\n",
    "2. Each trial results in one of two outcomes: success, $S$, or failure, $F$.\n",
    "3. The probability of success on a single trial is equal to some value $p$ and remains the same from trial to trial. The probability of a failure is equal to q = $(1 − p)$.\n",
    "4. The trials are independent.\n",
    "5. The random variable of interest is $Y$ , the number of successes observed during the $n$ trials."
   ]
  },
  {
   "cell_type": "markdown",
   "metadata": {},
   "source": [
    "Question 1: From the following steps shown above, derive the probability distribution of the experiment.\n",
    "\n",
    "Considering an experiment that consists of a set number of identical trials, denoted as $n$. In each trial, there are two possible outcomes: success, labeled as $S$, and failure, labeled as $F$. The probability of success in a single trial is a constant value $p$, and the probability of failure is $q=(1−p)$. These trials are independent of each other.\n",
    "\n",
    "The focus of our interest is the random variable $Y$, which represents the count of successes observed during the $n$ trials.\n",
    "\n",
    "Now, if we denote $k$ as the number of successes in $n$ trials, there are $(\\binom{n}{k})$ combinations of trials that can result in $k$ successes.\n",
    "\n",
    "Given the independence of trials, the likelihood of a specific sequence consisting of $k$ successes and $( n-k )$ failures is $( p^k q^{n-k} )$.\n",
    "\n",
    "The probability of witnessing exactly $k$ successes in $n$ trials is calculated by multiplying the number of sequences that yield $k$ successes by the likelihood of one such sequence. This gives us:\n",
    "\\begin{equation}\n",
    "P(Y = k) = \\binom{n}{k} p^k q^{n-k}\n",
    "\\end{equation}\n",
    "\n",
    "Since $q$ is the complement of $p$, we can substitute $( 1−p )$ for $q$ in the equation. This leads us to the probability distribution of the experiment:\n",
    "\\begin{equation}\n",
    "P(Y = k) = \\binom{n}{k} p^k (1 - p)^{n-k}\n",
    "\\end{equation}\n",
    "\n",
    "This equation is valid for all values of $k$ in the range of $ 0 $ to $n$. It represents the probability distribution of the experiment."
   ]
  },
  {
   "cell_type": "markdown",
   "metadata": {},
   "source": [
    "Question 2: Show that the expectation of this probability distribution is $E[y] = \\Sigma y \\cdotp P(y) = np$.\n",
    "\n",
    "We start with an experiment that consists of a fixed number, $n$, of identical trials. Each trial results in one of two outcomes: success, $S$, or failure, $F$. The probability of success on a single trial is equal to some value $p$ and remains the same from trial to trial. The probability of a failure is equal to $q=(1−p)$. The trials are independent. The random variable of interest is $Y$ , the number of successes observed during the $n$ trials. \n",
    "\n",
    "The expectation of this probability distribution is defined as $E[y] = \\Sigma_{y = 0}^n \\cdot P(y)$.\n",
    "\n",
    "We substitute the binomial probability mass function into the expectation, resulting in \n",
    "\n",
    "$E[y] = \\Sigma_{y = 0}^n \\cdotp \\binom{n}{y} \\cdot p^y \\cdot q^{n-y}$.\n",
    "\n",
    "Next, we simplify the expression by replacing $q$ with $(1−p)$ and rearranging terms, yielding \n",
    "\n",
    "$E[y] = \\Sigma_{y = 0}^n \\frac{n!}{y!(n-y)!} \\cdot (p)^y \\cdot (1-p)^{(n-y)}$.\n",
    "\n",
    "Since $p$ is constant, we can factor it out of the summation, giving \n",
    "\n",
    "$E[y] = np \\, \\Sigma_{y = 0}^n \\frac{(n-1)!}{(y-1)!(n-y)!} \\cdot (p)^{(y-1)} \\cdot (1-p)^{(n-y)}$.\n",
    "\n",
    "We then rearrange the terms to get \n",
    "\n",
    "$E[y] = np \\, \\Sigma_{y = 1}^n \\frac{(n-1)!}{(y-1)!(n-y)!} \\cdot (p)^{(y-1)} \\cdot (1-p)^{(n-y)}$.\n",
    " \n",
    "Applying the binomial theorem, which states that for any positive integers $n$ and $k$, one has the following equality:\n",
    "\n",
    "$(x+y)^{n}= \\Sigma_{k=0}^{n}\\binom{n}{k} x^{k} y^{n-k}$ \n",
    "\n",
    "where $\\binom{n}{k}$ denotes the binomial coefficient, we find that \n",
    "\n",
    "$(p + q)^ {n -1} = \\Sigma_{k = 0}^{n-1} \\binom{n-1}{y} \\cdot (p)^{(k)} \\cdot (q)^{(n-1-k)}$\n",
    "\n",
    "By comparing the terms in the expression to the binomial theorem, we can see that \n",
    "\n",
    "$(p + q)^ {n-1} = \\Sigma_{y = 0}^{n} \\frac{(n-1)!}{(y)!(n-y)!} \\cdot (p)^{(y)} \\cdot (q)^{(n-y)}$\n",
    "\n",
    "Finally, we simplify the expression. The expansion of $(p + (1-p))^{n-1}$ is simply $1^{n-1}$, which equals $1$. Therefore, the sum becomes $1$. This simplifies to $E[y] = np \\cdot 1$, which leads to the final simplification of $E[y] = np$.\n",
    "\n",
    "In conclusion, the expectation of a binomial distribution, $E[y] = np$, validates that the mean equals the product of the number of trials and the probability of success."
   ]
  },
  {
   "cell_type": "markdown",
   "metadata": {},
   "source": [
    "Question 3: Experience has shown that 30% of all persons afflicted by a certain illness recover. A drug company has developed a new medication. Ten people with the illness were selected at random and received the medication; nine recovered shortly thereafter. Suppose that the medication was absolutely worthless. What is the probability that at least nine of ten receiving the medication will recover?\n",
    "\n",
    "We’re considering a scenario where a drug company has developed a new medication for a certain illness. From past data, we know that 30% of all persons afflicted by this illness recover naturally, without any medication. This is our probability of success (recovery), denoted as $p=0.30$.\n",
    "\n",
    "In this case, ten people with the illness were selected at random and received the medication, and nine recovered shortly thereafter. We’re asked to calculate the probability that at least nine out of ten people receiving the medication will recover, assuming that the medication is absolutely worthless.\n",
    "\n",
    "We have a total of $n=10$ trials (people receiving the medication), and we’re interested in $y=9$ successes (recoveries).\n",
    "\n",
    "We can use the binomial probability mass function to calculate this probability. The binomial probability mass function gives us the probability of observing exactly $k$ successes in $n$ trials, and is given by:\n",
    "\n",
    "$P(Y=k) = \\binom{n}{k}p^k(1 - p)^{n-k}$\n",
    "\n",
    "In our case, we want to find the probability of observing at least 9 successes, so we need to calculate \n",
    "\n",
    "$P(Y \\geq 9) = P(Y = 9) + P(Y = 10)$\n",
    "\n",
    "Substituting the given values into the equation, we get:\n",
    "\n",
    "$P(Y \\geq 9) = \\binom{10}{9} \\cdot (0.30)^9 \\cdot (1 - 0.30)^{10-9} + \\binom{10}{10} \\cdot (1 - 0.30)^{10-10}$\n",
    "\n",
    "Simplifying this, we find:\n",
    "\n",
    "$ P(Y \\geq 9) = 10 \\cdot (0.30)^9 \\cdot 0.70 + (0.30)^{10}$\n",
    "\n",
    "This simplifies further to:\n",
    "\n",
    "$ P(Y \\geq 9) = 0.000137781 + 0.0000059049$\n",
    "\n",
    "Which sums up to:\n",
    "\n",
    "$ P (Y \\geq 9) \\approx 0.0001436869$ or $0.014 \\%$\n",
    "\n",
    "In conclusion, the probability that at least nine of ten receiving the medication will recover is approximately $0.0001436869$ or $0.014\\%$.\n"
   ]
  },
  {
   "cell_type": "markdown",
   "metadata": {},
   "source": [
    "Question 4: Suppose that a lot of 5000 electrical fuses contains 5% defectives. If a sample of 5 fuses is tested, find the probability of observing at least one defective.\n",
    "\n",
    "We’re looking for the probability of observing at least one defective fuse in a sample of 5, denoted as $P(Y \\geq 1)$.\n",
    "To find this, we can use the complement rule, which states that the probability of an event occurring is $1$ minus the probability of it not occurring. So, we need to calculate $P(Y=0)$, the probability of observing no defective fuses, and subtract it from $1$.\n",
    "\n",
    "The binomial probability formula is used to calculate $P(Y=0)$. This formula gives us the probability of observing exactly $k$ successes in $n$ trials, and is given by $P(Y=k)=\\binom{n}{k} \\times p^k  \\times q^{n−k}$.\n",
    "Here, $k=0$ (no defective fuses), $n=5$ (the number of fuses tested), $p=0.05$ (the probability of a fuse being defective), and $q=0.95$ (the probability of a fuse not being defective).\n",
    "\n",
    "Substituting these values into the equation, we get:\n",
    "\n",
    "$P(Y=0)= \\binom{5}{0} \\times 0.050 \\times 0.955$\n",
    "\n",
    "This simplifies to:\n",
    "\n",
    "$P(Y=0)=1 \\times 1 \\times (0.95)5=0.7737809375$\n",
    "\n",
    "Now, we can calculate $P(Y \\geq 1)$ as follows:\n",
    "\n",
    "$P(Y \\geq 1)=1−P(Y=0)=1−0.7737809375=0.2262190625$\n",
    "\n",
    "Therefore, the probability of observing at least one defective fuse in a sample of 5 is approximately $0.2262190625$, or $22.62\\%$"
   ]
  },
  {
   "cell_type": "markdown",
   "metadata": {},
   "source": [
    "Task 3: Consider a probility distribution of $p(y) = \\frac{\\lambda^y}{y!} e^{-\\lambda}$."
   ]
  },
  {
   "cell_type": "markdown",
   "metadata": {},
   "source": [
    "Question 1: Find a general formula for the expected value of this distribution.\n",
    "\n",
    "\n",
    "Given a probability distribution $p(y) = \\frac{\\lambda^y}{y!} e^{-\\lambda}$ and we want to find the expected value $E[Y]$ of this distribution. The expected value is the sum of all possible values of $Y$, each multiplied by their respective probabilities.\n",
    "\n",
    "So, we start with the formula for the expected value:\n",
    "\n",
    "$E[Y] = \\sum_{y=0}^{\\infty} y \\cdot p(y)$\n",
    "\n",
    "We then substitute the given probability distribution into this formula:\n",
    "\n",
    "$E[Y] = \\sum_{y=0}^{\\infty} y \\cdot \\frac{\\lambda^y}{y!} e^{-\\lambda}$\n",
    "\n",
    "Next, we simplify this expression by factoring out e−λ and shifting the index of the summation:\n",
    "\n",
    "$ E[Y] = \\sum_{y=0}^{\\infty} y \\cdot \\frac{\\lambda^y}{y!} e^{-\\lambda}$\n",
    "\n",
    "$E[Y] = e^{-\\lambda} \\sum_{y=0}^{\\infty} \\frac{\\lambda^y}{(y-1)!} $\n",
    "\n",
    "$E[Y] = e^{-\\lambda} \\sum_{y=1}^{\\infty} \\frac{\\lambda^y}{(y-1)!}$\n",
    "\n",
    "\n",
    "We then factor out $\\lambda$ from the summation:\n",
    "\n",
    "$E[Y] = e^{-\\lambda} \\lambda \\sum_{y=1}^{\\infty} \\frac{\\lambda^{y-1}}{(y-1)!}$\n",
    "\n",
    "And shift the index of the summation back to $0$:\n",
    "\n",
    "$E[Y] = e^{-\\lambda} \\lambda \\sum_{y=0}^{\\infty} \\frac{\\lambda^y}{y!}$\n",
    "\n",
    "At this point, we notice that the sum is the Taylor series expansion of $e^{\\lambda}$. Therefore, we can rewrite the sum as $e^{\\lambda}$:\n",
    "\n",
    "$ E[Y] = e^{-\\lambda} \\lambda e^{\\lambda}$\n",
    "\n",
    "Simplifying this expression, we get:\n",
    "\n",
    "$ E[Y] = \\lambda$\n",
    "\n",
    "Therefore, the general formula for the expected value of this distribution is $ E[Y] = \\lambda$. This means that on average, we would expect the outcome to be $\\lambda$ if we were to repeat the experiment many times."
   ]
  },
  {
   "cell_type": "markdown",
   "metadata": {},
   "source": [
    "\n",
    "Question 2: A certain type of tree has seedlings randomly dispersed in a large area, with the mean density of seedlings being approximately five per square yard. If a forester randomly locates ten 1-square-yard sampling regions in the area, find the probability that none of the regions will contain seedlings.\n",
    "\n",
    "This is a problem involving a Poisson distribution, which is given by the formula $ p(y) = \\frac{\\lambda^y}{y!} e^{-\\lambda} $. Here, $\\lambda$ is the average rate (mean density of seedlings per square yard), and $y$ is the number of seedlings in a region.\n",
    "\n",
    "Given that the mean density of seedlings is five per square yard, we have $\\lambda=5$.\n",
    "\n",
    "We want to find the probability that none of the regions will contain seedlings. This is the probability of having $y=0$ seedlings in a region. \n",
    "\n",
    "Substituting $\\lambda=5$ and $y=0$ into the Poisson distribution formula, we get \n",
    "\n",
    "$ p(0) = \\frac{5^0}{0!} e^{-5} = e^{-5} $.\n",
    "\n",
    "We can calculate this probability to be approximately \n",
    "$ p(0) \\approx e^{-5} \\approx 0.006737947 $.\n",
    "\n",
    "Therefore, the probability that none of the regions will contain seedlings is approximately $0.0067$, or $0.67\\%$. This means that it’s quite unlikely for a $1$-square-yard region to not contain any seedlings, given the high density of seedlings in the area."
   ]
  }
 ],
 "metadata": {
  "language_info": {
   "name": "python"
  }
 },
 "nbformat": 4,
 "nbformat_minor": 2
}
