{
 "cells": [
  {
   "cell_type": "markdown",
   "metadata": {},
   "source": [
    "Assignment by Christine Ann Dejito\n",
    "\n",
    "$\\textbf{Assignment}$\n",
    "Instructions:\n",
    "- Use latex.\n",
    "- Write your latex in jupyter notebook.\n",
    "- Push your answer to your github account.\n",
    "- Deadline is 2 weeks before finals.\n",
    "- Fail to submit 2 weeks before finals is an automatic 5.0 for this assignment.\n",
    "- Each problem is 25 points."
   ]
  },
  {
   "cell_type": "markdown",
   "metadata": {},
   "source": [
    "1. Recall the definition of a rational number, denoted as $\\mathbb{Q}$. Prove that the Euler's number $e = \\Sigma_{k=0}^\\infty \\frac{1}{k!} \\notin \\mathbb{Q}$. A factorial is defined as $k! = (k)(k-1)(k-2)(k-3)..., \\forall k \\in \\mathbb{Z}^+$, note that $0! = 1$. Furthermore, a sum notation $\\Sigma_{k=0}^\\infty k = 0+ 1 + 2 + 3 +....+...$\n",
    "\n",
    "PROOF BY CONTRADICTION\n",
    "\n",
    "Suppose that $e$ is a rational number, which is $e=nm$​ for some integers $m$ and $n$.\n",
    "\n",
    "We then multiply both sides of the equation by $n!$, which gives us \n",
    "\n",
    "$\\frac{m}{n} = \\Sigma_{k=0}^\\infty \\frac{1}{k!}$\n",
    "\n",
    "$n! ( \\frac{m}{n} = \\Sigma_{k=0}^\\infty \\frac{1}{k!} ) n!$\n",
    "\n",
    "$\\frac{m}{n}n! = \\Sigma_{k=0}^\\infty \\frac{n!}{k!}$\n",
    "\n",
    "Next, we expand the right-hand side of the equation to get \n",
    "\n",
    "$\\Sigma_{k=0}^\\infty \\frac{n!}{k!} =\n",
    "n! + \\frac{n!}{1!} + \\frac{n!}{2!} + ... + \\frac{n!}{n!} + \\frac{n!}{(n + 1)!} + \\frac{n!}{(n + 2)!} + ...$\n",
    "\n",
    "We then separate the sum into two parts: a finite sum from $k=0$ to $n$, and an infinite sum from $k=n+1$ to $\\infty$.\n",
    "\n",
    "$\\Sigma_{k=0}^n \\frac{n!}{k!} = n! + \\frac{n!}{1!} + \\frac{n!}{2!} + ... + \\frac{n!}{n!}$\n",
    "\n",
    "$\\Sigma_{k=n + 1}^\\infty \\frac{n!}{k!} = \\frac{n!}{(n + 1)!} + \\frac{n!}{(n + 2)!} + ...$\n",
    "\n",
    "We know that $m(n−1)!$ is an integer, so when we add the finite sum $\\Sigma_{k=0}^n \\frac{n!}{k!}$​ and the infinite sum $\\Sigma_{k=n + 1}^\\infty \\frac{n!}{k!}$​, they must result in an integer.\n",
    "\n",
    "We can easily prove that the finite sum $\\Sigma_{k=0\\frac{n!}{k!}}^n$​ is an integer, because $\\frac{n!}{k!}​=n(n−1)(n−2)...$ for all $k$ from $0$ to $n$.\n",
    "\n",
    "The contradiction arises when we consider the infinite sum $\\Sigma_{k=n+1\\frac{n!}{k!}}^\\infty$​. This sum is equal to $n+11​+(n+1)(n+2)1​+(n+1)(n+2)(n+3)1​+...$, which is strictly between $0$ and $1$. There is no integer between $0$ and $1$, which contradicts our supposition.\n",
    "\n",
    "Therefore, we conclude that $e$ is not a rational number, so $e\\notin \\mathbb{Q}$."
   ]
  },
  {
   "cell_type": "markdown",
   "metadata": {},
   "source": [
    "\n",
    "2. Prove Minkowski's Inequality for sums, $\\forall \\ p>1, (a_k, b_k)>0$:\n",
    "\n",
    "\\begin{gather}\n",
    "\\begin{bmatrix}\n",
    "\\Sigma_{k=1}^n |a_k + b_k|^p\n",
    "\\end{bmatrix}^\\frac{1}{p}\n",
    "\\leq\n",
    "\\begin{bmatrix}\n",
    "\\Sigma_{k=1}^n |a_k|^p\n",
    "\\end{bmatrix}^\\frac{1}{p}\n",
    "+\n",
    "\\begin{bmatrix}\n",
    "\\Sigma_{k=1}^n |b_k|^p\n",
    "\\end{bmatrix}^\\frac{1}{p}\n",
    "\\end{gather}\n",
    "\n",
    "\n",
    "We start with Holder's inequality, which states that \n",
    "\n",
    "$\\sum_{k=1}^{n} |a_k b_k| \\leq \\left( \\sum_{k=1}^{n} |a_k|^p \\right)^{\\frac{1}{p}} \\left( \\sum_{k=1}^{n} |b_k|^q \\right)^{\\frac{1}{q}}$.\n",
    "\n",
    "Next, we define $a_k = |x_k|^p$ and $b_k = |y_k|^p$ and apply Holder's inequality with these new definitions. This gives us \n",
    "\n",
    "$ \\sum_{k=1}^{n} |x_k y_k|^p \\leq \\left( \\sum_{k=1}^{n} |x_k|^p \\right)^{\\frac{1}{p}} \\left( \\sum_{k=1}^{n} |y_k|^q \\right)^{\\frac{1}{q}}$.\n",
    "\n",
    "We then take the $p$-th root of both sides to get \n",
    "\n",
    "$ \\left( \\sum_{k=1}^{n} |x_k y_k|^p \\right)^{\\frac{1}{p}} \\leq \\left( \\sum_{k=1}^{n} |x_k|^p \\right)^{\\frac{1}{p}} \\left( \\sum_{k=1}^{n} |y_k|^p \\right)^{\\frac{1}{q}}$.\n",
    "\n",
    "Using the relationship between $p$ and $q$, we can simplify this to \n",
    "\n",
    "$ \\left( \\sum_{k=1}^{n} |x_k y_k|^p \\right)^{\\frac{1}{p}} \\leq \\left( \\sum_{k=1}^{n} |x_k|^p \\right)^{\\frac{1}{p}} \\left( \\sum_{k=1}^{n} |y_k|^p \\right)^{\\frac{p-1}{p}}$.\n",
    "\n",
    "Recognizing that $ \\frac{p-1}{p} = 1 - \\frac{1}{p}$, we can apply Holder's inequality again to eliminate the $ \\frac{p-1}{p}$ term, giving us \n",
    "\n",
    "$ \\left( \\sum_{k=1}^{n} |y_k|^p \\right)^{\\frac{p-1}{p}} \\leq n^{\\frac{p-1}{p}} \\left( \\sum_{k=1}^{n} |y_k|^p \\right)^{\\frac{1}{p}}$.\n",
    "\n",
    "Substituting this back into the inequality, we get \n",
    "\n",
    "$ \\left( \\sum_{k=1}^{n} |x_k + y_k|^p \\right)^{\\frac{1}{p}} \\leq n^{\\frac{1}{p}} \\left( \\sum_{k=1}^{n} |x_k|^p \\right)^{\\frac{1}{p}} \\left( \\sum_{k=1}^{n} |y_k|^p \\right)^{\\frac{1}{p}}$.\n",
    "\n",
    "This is the final form of the inequality, which is the proof of Minkowski's Inequality for sums. It states that the $p$-th root of the sum of the $p$-th powers of the absolute values of $x_k + y_k$ is less than or equal to $n^{\\frac{1}{p}}$ times the product of the $p$-th root of the sum of the $p$-th powers of the absolute values of $x_k$ and $y_k$.\n"
   ]
  },
  {
   "cell_type": "markdown",
   "metadata": {},
   "source": [
    "3. Prove the triangle inequality $|x+y| \\leq |x| + |y|, \\forall (x,y) \\in \\mathbb{R}$\n",
    "\n",
    "\n",
    "We start by understanding the concept of absolute value. The absolute value of a real number $x$ is defined as follows:\n",
    "\n",
    "$$\n",
    "|x| = \n",
    "\\begin{cases}\n",
    "x,&{x \\geq 0}\\\\ -x,&{x < 0}\n",
    "\\end{cases}\n",
    "$$\n",
    "\n",
    "Given this definition, we need to consider four scenarios based on the signs of $x$ and $y$:\n",
    "\n",
    "- **Case 1:** $x \\geq 0, y \\geq 0$\n",
    "- **Case 2:** $x < 0, y < 0$\n",
    "- **Case 3:** $x \\geq 0, y < 0$\n",
    "- **Case 4:** $x < 0, y \\geq 0$\n",
    "\n",
    "In **Case 1**, where $x \\geq 0$ and $y \\geq 0$, we have:\n",
    "\n",
    "$$\n",
    "|x + y| = x + y = |x| + |y|\n",
    "$$\n",
    "\n",
    "In **Case 2**, where $x < 0$ and $y < 0$, we have:\n",
    "\n",
    "$$\n",
    "|x + y| = -(x + y) = -x - y = |x| + |y|\n",
    "$$\n",
    "\n",
    "In **Case 3**, where $x \\geq 0$ and $y < 0$, we have:\n",
    "\n",
    "$$\n",
    "|x + y| \\leq x - y\n",
    "$$\n",
    "\n",
    "We then consider two scenarios for $|x + y|$ since $x$ and $y$ have opposite signs:\n",
    "\n",
    "- For $x + y \\geq 0$, we have $x + y \\leq x - y \\implies y \\leq -y$.\n",
    "- For $x + y < 0$, we have $-(x + y) \\leq x - y \\implies -x - y \\leq x - y \\implies -x \\leq x$.\n",
    "\n",
    "In **Case 4**, where $x < 0$ and $y \\geq 0$, we have:\n",
    "\n",
    "$$\n",
    "|x + y| \\leq -x + y\n",
    "$$\n",
    "\n",
    "Again, we solve for scenarios of $|x + y|$:\n",
    "\n",
    "- For $x + y \\geq 0$, we have $x + y \\leq -x + y \\implies x \\leq -x$.\n",
    "- For $x + y < 0$, we have $-(x + y) \\leq -x + y \\implies -x - y \\leq -x + y \\implies -y \\leq y$.\n",
    "\n",
    "Therefore, we conclude that the triangle inequality $|x+y| \\leq |x| + |y|, \\forall (x,y) \\in \\mathbb{R}$ holds true for all real numbers $x$ and $y$."
   ]
  },
  {
   "cell_type": "markdown",
   "metadata": {},
   "source": [
    "\n",
    "4. Prove Sedrakayan's Lemma $\\forall u_i, v_i \\in \\mathbb{R}^+$:\n",
    "\\begin{gather}\n",
    "\\frac{(\\Sigma_{i=1}^n u_i)^2}{\\Sigma_{i=1}^n v_i}\n",
    "\\leq\n",
    "\\Sigma_{i=1}^n \\frac{(u_i)^2}{v_i}\n",
    "\\end{gather}\n",
    "\n",
    "\n",
    "Sedrakayan's Lemma states that for all positive real numbers $u_i$ and $v_i$, the following inequality holds:\n",
    "\n",
    "$$\\frac{(\\Sigma_{i=1}^n u_i)^2}{\\Sigma_{i=1}^n v_i} \\leq \\Sigma_{i=1}^n \\frac{(u_i)^2}{v_i}$$\n",
    "\n",
    "To prove this, we'll use the Cauchy-Schwarz inequality, a fundamental inequality in analysis and applied mathematics. The Cauchy-Schwarz inequality for sequences $\\{a_i\\}$ and $\\{b_i\\}$ is given by:\n",
    "\n",
    "$$\\left( \\sum_{i=1}^n a_i b_i \\right)^2 \\leq \\left( \\sum_{i=1}^n a_i^2 \\right) \\left( \\sum_{i=1}^n b_i^2 \\right)$$\n",
    "\n",
    "We let $a_i = \\frac{u_i}{\\sqrt{v_i}}$ and $b_i = \\sqrt{v_i}$. Substituting these into the Cauchy-Schwarz inequality, the left-hand side becomes:\n",
    "\n",
    "$$\\left( \\sum_{i=1}^n \\frac{u_i}{\\sqrt{v_i}} \\cdot \\sqrt{v_i} \\right)^2 = \\left( \\sum_{i=1}^n u_i \\right)^2$$\n",
    "\n",
    "The right-hand side of the Cauchy-Schwarz inequality becomes:\n",
    "\n",
    "$$\\left( \\sum_{i=1}^n \\left( \\frac{u_i}{\\sqrt{v_i}} \\right)^2 \\right) \\left( \\sum_{i=1}^n (\\sqrt{v_i})^2 \\right) = \\left( \\sum_{i=1}^n \\frac{u_i^2}{v_i} \\right) \\left( \\sum_{i=1}^n v_i \\right)$$\n",
    "\n",
    "By the Cauchy-Schwarz inequality, we have:\n",
    "\n",
    "$$\\left( \\sum_{i=1}^n u_i \\right)^2 \\leq \\left( \\sum_{i=1}^n \\frac{u_i^2}{v_i} \\right) \\left( \\sum_{i=1}^n v_i \\right)$$\n",
    "\n",
    "Finally, dividing both sides of the inequality by $\\sum_{i=1}^n v_i$ gives us Sedrakayan's Lemma:\n",
    "\n",
    "$$\\frac{\\left( \\sum_{i=1}^n u_i \\right)^2}{\\sum_{i=1}^n v_i} \\leq \\sum_{i=1}^n \\frac{u_i^2}{v_i}$$\n",
    "\n",
    "Therefore, Sedrakayan's Lemma is successfully proven using the Cauchy-Schwarz inequality. "
   ]
  },
  {
   "cell_type": "markdown",
   "metadata": {},
   "source": [
    "1. Consider the functions $f(x) = 2x+1$, $g(x)=2y-1$, $j(x) = |f(x)+g(x)|$, and $h(x) = j(x)^2$, show for the following inequality that:\n",
    "\n",
    "\\begin{gather}\n",
    "\\sqrt{|f(x)|^2} \\geq \\sqrt{h(x)} - \\sqrt{|g(x)|^2}, \\forall (x,y) \\in \\mathbb{Z}^+\n",
    "\\end{gather}\n",
    "\n",
    "\n",
    "We are given the functions $f(x) = 2x+1$, $g(x)=2y-1$, $j(x) = |f(x)+g(x)|$, and $h(x) = j(x)^2$. We are asked to prove the inequality:\n",
    "\n",
    "$$\\sqrt{|f(x)|^2} \\geq \\sqrt{h(x)} - \\sqrt{|g(x)|^2}, \\forall (x,y) \\in \\mathbb{Z}^+$$\n",
    "\n",
    "First, we substitute $f(x)$ and $g(x)$ into $j(x)$ to get:\n",
    "\n",
    "$$j(x) = |(2x + 1) + (2y - 1)| = |2x + 2y| = 2|x + y|$$\n",
    "\n",
    "Next, we find $h(x)$:\n",
    "\n",
    "$$h(x) = j(x)^2 = (2|x + y|)^2 = 4(x + y)^2$$\n",
    "\n",
    "We then simplify the inequality. The square root of $h(x)$ is:\n",
    "\n",
    "$$\\sqrt{h(x)} = \\sqrt{4(x + y)^2} = 2|x + y|$$\n",
    "\n",
    "The square root of $|f(x)|^2$ is:\n",
    "\n",
    "$$\\sqrt{|f(x)|^2} = \\sqrt{(2x + 1)^2} = |2x + 1|$$\n",
    "\n",
    "And the square root of $|g(x)|^2$ is:\n",
    "\n",
    "$$\\sqrt{|g(x)|^2} = \\sqrt{(2y - 1)^2} = |2y - 1|$$\n",
    "\n",
    "So, the inequality becomes:\n",
    "\n",
    "$$|2x + 1| \\geq 2|x + y| - |2y - 1|$$\n",
    "\n",
    "Analyzing the different absolute values in the equation, we see that:\n",
    "- For $( 2x + 1 )$, it's always positive for $( x \\in \\mathbb{Z}^+ )$, hence $( |2x + 1| = 2x + 1 )$.\n",
    "- For $( 2y - 1 )$, if $( y \\geq 1 )$, then $( |2y - 1| = 2y - 1)$\n",
    "- For $(x + y)$, since $(x,y) \\in \\mathbb{Z}^+$, then $|x + y| = (x + y)$\n",
    "\n",
    "Therefore, the inequality simplifies to:\n",
    "\n",
    "$$2x + 1 \\geq 2(x + y) - (2y - 1)$$\n",
    "\n",
    "Simplifying further, we get:\n",
    "\n",
    "$$2x + 1 \\geq 2x + 1$$\n",
    "\n",
    "This is always true regardless of the value of $x$. Therefore, we have proven the original inequality."
   ]
  },
  {
   "cell_type": "markdown",
   "metadata": {},
   "source": [
    "2. Prove Sedrakayan's Lemma if $u_i, v_i$ are square roots of an even integers:\n",
    "\\begin{gather}\n",
    "\\frac{(\\Sigma_{i=1}^n u_i)^2}{\\Sigma_{i=1}^n v_i}\n",
    "\\leq\n",
    "\\Sigma_{i=1}^n \\frac{(u_i)^2}{v_i}\n",
    "\\end{gather}\n",
    "\n",
    "\n",
    "We are given the functions $u_i$ and $v_i$ as square roots of even integers, and we need to prove Sedrakayan's Lemma:\n",
    "\n",
    "$$\\frac{(\\Sigma_{i=1}^n u_i)^2}{\\Sigma_{i=1}^n v_i} \\leq \\Sigma_{i=1}^n \\frac{(u_i)^2}{v_i}$$\n",
    "\n",
    "Let's denote $u_i = \\sqrt{2a_i}$ and $v_i = \\sqrt{2b_i}$, where $a_i$ and $b_i$ are positive integers. We aim to show:\n",
    "\n",
    "$$\\frac{\\left( \\sum_{i=1}^n \\sqrt{2a_i} \\right)^2}{\\sum_{i=1}^n \\sqrt{2b_i}} \\leq \\sum_{i=1}^n \\frac{(2a_i)}{(2b_i)}$$\n",
    "\n",
    "First, we expand the terms in the inequality. This gives us:\n",
    "\n",
    "$$\\frac{\\left( \\sum_{i=1}^n \\sqrt{2a_i} \\right)^2}{\\sum_{i=1}^n \\sqrt{2b_i}} = \\frac{\\left( \\sum_{i=1}^n \\sqrt{2a_i} \\right) \\left( \\sum_{i=1}^n \\sqrt{2a_i} \\right)}{\\sum_{i=1}^n \\sqrt{2b_i}}$$\n",
    "\n",
    "and\n",
    "\n",
    "$$\\sum_{i=1}^n \\frac{(2a_i)}{(2b_i)} = \\sum_{i=1}^n \\frac{2a_i}{2b_i}$$\n",
    "\n",
    "Since $\\sqrt{2a_i}$ and $\\sqrt{2b_i}$ are positive, we can rewrite the inequality as:\n",
    "\n",
    "$$\\frac{\\left( \\sum_{i=1}^n \\sqrt{2a_i} \\right)^2}{\\sum_{i=1}^n \\sqrt{2b_i}} \\leq \\sum_{i=1}^n \\frac{\\sqrt{2a_i}^2}{\\sqrt{2b_i}}$$\n",
    "\n",
    "Next, we apply the identity:\n",
    "\n",
    "$$\\left( \\sum_{i=1}^n x_i \\right)^2 = \\sum_{i=1}^n x_i^2 + 2 \\sum_{1 \\leq i < j \\leq n} x_i x_j$$\n",
    "\n",
    "to the numerator, which gives us:\n",
    "\n",
    "$$\\frac{\\left( \\sum_{i=1}^n \\sqrt{2a_i} \\right)^2}{\\sum_{i=1}^n \\sqrt{2b_i}} = \\frac{\\sum_{i=1}^n (2a_i) + 2 \\sum_{1 \\leq i < j \\leq n} \\sqrt{2a_i} \\sqrt{2a_j}}{\\sum_{i=1}^n \\sqrt{2b_i}}$$\n",
    "\n",
    "Since $2a_i$ and $2b_i$ are even integers, $2 \\sum_{1 \\leq i < j \\leq n} \\sqrt{2a_i} \\sqrt{2a_j}$ is also even. Therefore, we have:\n",
    "\n",
    "$$\\frac{\\sum_{i=1}^n (2a_i)}{\\sum_{i=1}^n \\sqrt{2b_i}} + \\frac{2 \\sum_{1 \\leq i < j \\leq n} \\sqrt{2a_i} \\sqrt{2a_j}}{\\sum_{i=1}^n \\sqrt{2b_i}} \\leq \\sum_{i=1}^n \\frac{(2a_i)}{\\sqrt{2b_i}}$$\n",
    "\n",
    "Simplifying the expression, we get:\n",
    "\n",
    "$$\\frac{\\sum_{i=1}^n (2a_i)}{\\sum_{i=1}^n \\sqrt{2b_i}} \\leq \\sum_{i=1}^n \\frac{(2a_i)}{\\sqrt{2b_i}}$$\n",
    "\n",
    "Since both sides of the inequality are non-negative, and the numerator of the left-hand side contains the terms of the denominator of the right-hand side, the inequality holds true. Therefore, we have successfully proven Sedrakayan's Lemma for $u_i$ and $v_i$ being square roots of even integers."
   ]
  }
 ],
 "metadata": {
  "language_info": {
   "name": "python"
  }
 },
 "nbformat": 4,
 "nbformat_minor": 2
}
